Cleanup Weakening, move on_free_vars to a separate library

pcuic/theories/PCUICRename.v
@@ -4,7 +4,7 @@ From MetaCoq.Template Require Import config utils.
 From MetaCoq.PCUIC Require Import PCUICAst PCUICAstUtils PCUICCases PCUICInduction
   PCUICLiftSubst PCUICUnivSubst
   PCUICTyping PCUICClosed PCUICEquality PCUICWeakeningEnv
-  PCUICSigmaCalculus PCUICClosed.
+  PCUICSigmaCalculus PCUICClosed PCUICOnFreeVars.
 
 Require Import ssreflect ssrbool.
 From Equations Require Import Equations.
@@ -17,11 +17,6 @@ Open Scope sigma_scope.
 Set Keyed Unification.
 
 Set Default Goal Selector "!".
-
-Tactic Notation "relativize" open_constr(c) := 
-  let ty := type of c in  
-  let x := fresh in
-  evar (x : ty); replace c with x; subst x.
 
 Lemma rename_mkApps :
   forall f t l,
@@ -269,21 +264,17 @@ Definition urenaming (P : nat -> bool) Γ Δ f :=
       on_Some_or_None (fun body => Some (rename (f ∘ rshiftk (S i)) body) =
          option_map (rename (rshiftk (S (f i)))) decl'.(decl_body)) decl.(decl_body))).
 
-(* Definition urenaming (P : nat -> bool) Γ Δ f :=
-  forall i decl,
-    P i ->
-    nth_error Δ i = Some decl ->
-    ∑ decl',
-      nth_error Γ (f i) = Some decl' ×
-      eq_binder_annot decl.(decl_name) decl'.(decl_name) ×
-      rename f (lift0 (S i) decl.(decl_type))
-      = lift0 (S (f i)) decl'.(decl_type) ×
-      (forall b,
-         decl.(decl_body) = Some b ->
-         ∑ b',
-           decl'.(decl_body) = Some b' ×
-           rename f (lift0 (S i) b) = lift0 (S (f i)) b'
-      ). *)
+Lemma urenaming_impl :
+  forall (P P' : nat -> bool) Γ Δ f,
+    (forall i, P' i -> P i) ->
+    urenaming P Δ Γ f ->
+    urenaming P' Δ Γ f.
+Proof.
+  intros P P' Γ Δ f hP h.
+  intros i decl p e.
+  specialize (h i decl (hP _ p) e) as [decl' [h1 [h2 h3]]].
+  exists decl'. split ; [| split ]; eauto.
+Qed.
 
 (* Definition of a good renaming with respect to typing *)
 Definition renaming P Σ Γ Δ f :=
@@ -334,6 +325,17 @@ Proof.
     simpl. reflexivity.
 Qed.
 
+Lemma rename_closed :
+  forall f t,
+    closed t ->
+    rename f t = t.
+Proof.
+  intros f t h.
+  replace (rename f t) with (rename (shiftn 0 f) t).
+  - apply rename_closedn. assumption.
+  - now sigma.
+Qed.
+
 Lemma rename_closed_decl k f d : closed_decl k d -> map_decl (rename (shiftn k f)) d = d.
 Proof.
   rewrite /closed_decl /map_decl.  
@@ -367,42 +369,6 @@ Proof.
   intros cl. apply rename_closedn_terms.
   now apply (closedn_extended_subst_gen Γ 0 0).
 Qed.
-
-(* TODO MOVE *)
-Lemma rename_closed :
-  forall f t,
-    closed t ->
-    rename f t = t.
-Proof.
-  intros f t h.
-  replace (rename f t) with (rename (shiftn 0 f) t).
-  - apply rename_closedn. assumption.
-  - now sigma.
-Qed.
-
-(* TODO MOVE *)
-Lemma declared_constant_closed_body :
-  forall Σ cst decl body,
-    wf Σ ->
-    declared_constant Σ cst decl ->
-    decl.(cst_body) = Some body ->
-    closed body.
-Proof.
-  intros Σ cst decl body hΣ h e.
-  unfold declared_constant in h.
-  eapply lookup_on_global_env in h. 2: eauto.
-  destruct h as [Σ' [wfΣ' decl']].
-  red in decl'. red in decl'.
-  destruct decl as [ty bo un]. simpl in *.
-  rewrite e in decl'.
-  now eapply subject_closed in decl'.
-Qed.
-
-Definition shiftnP k p i :=
-  if i <? k then true else p (i - k).
-
-Instance shiftnP_ext k : Proper (`=1` ==> `=1`) (shiftnP k).
-Proof. intros f g Hfg i. now rewrite /shiftnP Hfg. Qed. 
 
 Arguments Nat.sub !_ !_.
 
@@ -504,15 +470,14 @@ Proof.
     now setoid_rewrite <- (hfg _).
 Qed.
 
-(* Instance urename_proper : CMorphisms.Proper (`=1` ==> Logic.eq ==> Logic.eq ==> `=1` ==> CRelationClasses.iffT) urenaming.
+Lemma renaming_extP P P' Σ Γ Δ f :
+  P =1 P' ->
+  renaming P Σ Γ Δ f -> renaming P' Σ Γ Δ f.
 Proof.
-  intros P P' Hpp' ? ? -> ? ? -> f g Hfg. *)
-
-Lemma shiftnP0 P : shiftnP 0 P =1 P.
-Proof. rewrite /shiftnP. intros i; rewrite Nat.sub_0_r //. Qed.
-
-Lemma shiftnP_add n k P : shiftnP n (shiftnP k P) =1 shiftnP (n + k) P.
-Proof. rewrite /shiftnP. intros i; repeat nat_compare_specs => //. lia_f_equal. Qed.
+  intros hP; rewrite /renaming.
+  intros []; split; eauto.
+  eapply urenaming_ext; eauto. reflexivity.
+Qed.
 
 Lemma urenaming_context :
   forall P Γ Δ Ξ f,
@@ -763,7 +728,6 @@ Proof.
   apply IHn.
 Qed.
 
-
 Instance rename_context_ext : Proper (`=1` ==> Logic.eq ==> Logic.eq) rename_context.
 Proof.
   intros f g Hfg x y ->.
@@ -832,9 +796,6 @@ Proof.
   rewrite rename_context_subst_k rename_inds. now len.
 Qed.
 
-Definition map_pair {A B C D} (f : A -> B) (g : C -> D) (p : A × C) : B × D :=
-  (f p.1, g p.2).
-
 Lemma rename_reln f ctx n acc :
   forallb (closedn (n + #|ctx|)) acc ->
   map (rename (shiftn (n + #|ctx|) f)) (reln acc n ctx) = 
@@ -859,31 +820,12 @@ Proof.
   now apply (rename_reln _ _ 0).
 Qed.
 
-Lemma reln_fold f ctx n acc :
-  reln acc n (fold_context f ctx) = 
-  reln acc n ctx.
-Proof.
-  induction ctx as [|[na [b|] ty] ctx] in n, acc |- *; simpl; auto;
-    rewrite fold_context_snoc0 /=; apply IHctx.
-Qed.
-
 Lemma to_extended_list_rename f ctx :
   to_extended_list (rename_context f ctx) = to_extended_list ctx.
 Proof.
   unfold to_extended_list, to_extended_list_k.
   now rewrite (reln_fold _ _ 0).
 Qed.
-
-(* 
-Lemma rename_context_expand_lets_ctx k f Γ Δ :
-  k = context_assumptions Γ ->
-  rename_context (shiftn k f) (expand_lets_ctx Γ Δ) =
-  expand_lets_ctx (
-
-Lemma rename_context_expand_lets_ctx k f Γ Δ :
-  k = context_assumptions Γ ->
-  rename_context (shiftn k f) (expand_lets_ctx Γ Δ) =
-  expand_lets_ctx () *)
 
 Lemma rename_case_predicate_context {Σ} {wfΣ : wf Σ} {ind mdecl idecl f p} :
   declared_inductive Σ ind mdecl idecl ->
@@ -1109,381 +1051,11 @@ Proof.
        now rewrite /to_extended_list /to_extended_list_k reln_fold.
 Qed.
 
-Fixpoint all_free_vars (p : nat -> bool) (t : term) : bool :=
-  match t with
-  | tRel i => p i
-  | tEvar ev args => List.forallb (all_free_vars p) args
-  | tLambda _ T M | tProd _ T M => all_free_vars p T && all_free_vars (shiftnP 1 p) M
-  | tApp u v => all_free_vars p u && all_free_vars p v
-  | tLetIn na b t b' => [&& all_free_vars p b, all_free_vars p t & all_free_vars (shiftnP 1 p) b']
-  | tCase ind pred c brs =>
-    [&& forallb (all_free_vars p) pred.(pparams),
-      all_free_vars (shiftnP #|pred.(pcontext)| p) pred.(preturn),
-      all_free_vars p c &
-      forallb (fun br => all_free_vars (shiftnP #|br.(bcontext)| p) br.(bbody)) brs]
-  | tProj _ c => all_free_vars p c
-  | tFix mfix idx | tCoFix mfix idx =>
-    List.forallb (test_def (all_free_vars p) (all_free_vars (shiftnP #|mfix| p))) mfix
-  | tVar _ | tSort _ | tConst _ _ | tInd _ _ | tConstruct _ _ _ 
-  | tPrim _ => true
-  end.
-
-Lemma all_free_vars_ext (p q : nat -> bool) t : 
-  p =1 q ->
-  all_free_vars p t = all_free_vars q t.
-Proof.
-  revert p q.
-  induction t using PCUICInduction.term_forall_list_ind; simpl => //; intros;
-    unfold test_def;
-    rewrite ?forallb_map; try eapply All_forallb_eq_forallb; tea; eauto 2.
-  all: try now rewrite (IHt1 p q) // ?(IHt2 (shiftnP 1 p) (shiftnP 1 q)) // H.
-  - now rewrite (IHt1 p q) // ?(IHt2 p q) // (IHt3 (shiftnP 1 p) (shiftnP 1 q)) // H.
-  - rewrite (IHt1 p q) // (IHt2 p q) //.
-  - destruct X. red in X0.
-    f_equal.
-    * eapply All_forallb_eq_forallb; tea. solve_all.
-    * f_equal; [eapply e; rewrite H //|].
-      f_equal; [eapply IHt; rewrite H //|].
-      eapply All_forallb_eq_forallb; tea. intros.
-      eapply H0; rewrite H //.
-  - simpl; intuition auto. f_equal; eauto 2.
-    eapply b; rewrite H //.
-  - simpl; intuition auto. f_equal; eauto 2.
-    eapply b; rewrite H //.
-Qed.
-
-Instance all_free_vars_proper : Proper (`=1` ==> Logic.eq ==> Logic.eq) all_free_vars.
-Proof. intros f g Hfg ? ? ->. now apply all_free_vars_ext. Qed.
-
-Instance all_free_vars_proper_pointwise : Proper (`=1` ==> `=1`) all_free_vars.
-Proof. intros f g Hfg x. now apply all_free_vars_ext. Qed.
-
-Lemma shiftnP_impl (p q : nat -> bool) : (forall i, p i -> q i) ->
-  forall n i, shiftnP n p i -> shiftnP n q i.
-Proof.
-  intros Hi n i. rewrite /shiftnP.
-  nat_compare_specs => //. apply Hi.
-Qed.
-
-Lemma all_free_vars_impl (p q : nat -> bool) t : (forall i, p i -> q i) -> 
-  all_free_vars p t -> all_free_vars q t.
-Proof.
-  revert t p q.
-  induction t using PCUICInduction.term_forall_list_ind; simpl => //; solve_all.
-  all:try (rtoProp; now rewrite ?IHt1 ?IHt2 ?IHt3; eauto 2).
-  - rtoProp. intuition auto.
-    * eapply IHt1; eauto.
-    * eapply IHt2; eauto using shiftnP_impl.
-  - rtoProp; intuition auto.
-    * eapply IHt1; eauto.
-    * eapply IHt2; eauto using shiftnP_impl.
-  - rtoProp; intuition eauto 3 using shiftnP_impl.
-  - rtoProp; intuition eauto 3 using shiftnP_impl.
-    * solve_all.
-    * solve_all; eauto using shiftnP_impl.
-  - unfold test_def in *. apply /andP. move/andP: b. intuition eauto using shiftnP_impl.
-  - unfold test_def in *. apply /andP. move/andP: b. intuition eauto using shiftnP_impl.
-Qed.
-
-Definition closedP (n : nat) (P : nat -> bool) := 
-  fun i => if i <? n then P i else false.
-  
-Instance closedP_proper n : Proper (`=1` ==> `=1`) (closedP n).
-Proof. intros f g Hfg. intros i; rewrite /closedP. now rewrite Hfg. Qed.
-  
-Lemma shiftnP_closedP k n P : shiftnP k (closedP n P) =1 closedP (k + n) (shiftnP k P).
-Proof.
-  intros i; rewrite /shiftnP /closedP.
-  repeat nat_compare_specs => //.
-Qed.
-
-Lemma shiftnP_xpredT n : shiftnP n xpredT =1 xpredT.
-Proof. intros i; rewrite /shiftnP. nat_compare_specs => //. Qed.
-
-Lemma closedP_all_free_vars {n t} : closedn n t -> all_free_vars (closedP n xpredT) t.
-Proof.
-  revert n t.
-  apply: term_closedn_list_ind; simpl => //; intros.
-  all:(rewrite ?shiftnP_closedP ?shiftnP_xpredT).
-  all:try (rtoProp; now rewrite ?IHt1 ?IHt2 ?IHt3).
-  - rewrite /closedP /=. now nat_compare_specs.
-  - solve_all.
-  - destruct X. rtoProp. intuition solve_all.
-    now rewrite shiftnP_closedP shiftnP_xpredT.
-  - unfold test_def. solve_all.
-    rewrite a. rewrite shiftnP_closedP shiftnP_xpredT.
-    now len in b.
-  - unfold test_def; solve_all. 
-    rewrite a. rewrite shiftnP_closedP shiftnP_xpredT.
-    now len in b.
-Qed.
-
-Lemma closedn_all_free_vars {P n t} : closedn n t -> all_free_vars (shiftnP n P) t.
-Proof.
-  move/closedP_all_free_vars.
-  eapply all_free_vars_impl.
-  intros i; rewrite /closedP /shiftnP /= //.
-  nat_compare_specs => //.
-Qed.
-
-(** Any predicate is admissible as there are no free variables to consider *)
-Lemma closed_all_free_vars {P t} : closed t -> all_free_vars P t.
-Proof.
-  move/closedP_all_free_vars.
-  eapply all_free_vars_impl.
-  intros i; rewrite /closedP /= //.
-Qed.
-
-Lemma all_free_vars_subst_instance {p u t} : all_free_vars p t = all_free_vars p (subst_instance_constr u t).
-Proof.
-  revert t p.
-  apply: term_forall_list_ind; simpl => //; intros.
-  all:try (rtoProp; now rewrite -?IHt1 -?IHt2 -?IHt3).
-  - rewrite forallb_map. eapply All_forallb_eq_forallb; eauto.
-  - destruct X. f_equal.
-    * rewrite forallb_map; eapply All_forallb_eq_forallb; eauto.
-    * rewrite -e -H. f_equal. f_equal.
-      rewrite forallb_map. eapply All_forallb_eq_forallb; eauto.
-  - unfold test_def. rewrite forallb_map; len.
-    eapply All_forallb_eq_forallb; intuition eauto. solve_all.
-  - unfold test_def; rewrite forallb_map; len.
-    eapply All_forallb_eq_forallb; intuition eauto. solve_all.
-Qed.
-
-Definition test_decl (f : term -> bool) (d : context_decl) : bool :=
-  f d.(decl_type) && foroptb f d.(decl_body).
-
-Instance foroptb_proper A : Proper (`=1` ==> Logic.eq ==> Logic.eq) (@foroptb A).
-Proof.
-  intros f g Hfg x y ->; rewrite /foroptb.
-  destruct y; simpl; rewrite // ?Hfg.
-Qed.
-
-Instance foroptb_proper_pointwise A : Proper (`=1` ==> `=1`) (@foroptb A).
-Proof.
-  intros f g Hfg y; rewrite /foroptb.
-  destruct y; simpl; rewrite // ?Hfg.
-Qed.
-
-Instance test_decl_proper : Proper (`=1` ==> Logic.eq ==> Logic.eq) test_decl.
-Proof. 
-  intros f g Hfg [na [b|] ty] ? <- => /=; rewrite /test_decl /=;
-  now rewrite Hfg.
-Qed.
-
-Definition all_free_vars_decl P d :=
-  test_decl (all_free_vars P) d.
-
-Instance all_free_vars_decl_proper : Proper (`=1` ==> Logic.eq ==> Logic.eq) all_free_vars_decl.
-Proof. rewrite /all_free_vars_decl => f g Hfg x y <-. now rewrite Hfg. Qed.
-
-Instance all_free_vars_decl_proper_pointwise : Proper (`=1` ==> `=1`) all_free_vars_decl.
-Proof. rewrite /all_free_vars_decl => f g Hfg x. now rewrite Hfg. Qed.
-
-Definition all_free_vars_ctx P ctx :=
-  alli (fun k => (all_free_vars_decl (shiftnP k P))) 0 (List.rev ctx).
-
-Instance all_free_vars_ctx_proper : Proper (`=1` ==> `=1`) all_free_vars_ctx.
-Proof.
-  rewrite /all_free_vars_ctx => f g Hfg x.
-  now setoid_rewrite Hfg. 
-Qed.
-
-Definition orP (p q : nat -> bool) (n : nat) : bool :=
-  p n || q n.
-
-Definition conjP (p q : nat -> bool) (n : nat) : bool :=
-  p n && q n.
-
-Definition implP (p q : nat -> bool) (n : nat) : bool :=
-  p n ==> q n.
-
-Lemma alli_impl {A} (p q : nat -> A -> bool) n (l : list A) : 
-  (forall i x, p i x -> q i x) ->
-  alli p n l -> alli q n l.
-Proof.
-  intros hpq. induction l in n |- *; simpl; auto.
-  move/andP => [pna a'].
-  rewrite (hpq _ _ pna).
-  now apply IHl.
-Qed.
-
-Lemma test_decl_impl (p q : term -> bool) d : 
-  (forall i, p i -> q i) -> 
-  test_decl p d -> test_decl q d.
-Proof.
-  intros hp. unfold test_decl.
-  move/andP => [hty hbody].
-  rewrite hp //.
-  unfold foroptb in *.
-  destruct (decl_body d) => // /=.
-  now rewrite (hp _ hbody).
-Qed.
-
-Lemma all_free_vars_decl_impl (p q : nat -> bool) d : 
-  (forall i, p i -> q i) -> 
-  all_free_vars_decl p d -> all_free_vars_decl q d.
-Proof.
-  intros hpi.
-  apply test_decl_impl. intros t.
-  now apply all_free_vars_impl.
-Qed.
-
-Lemma all_free_vars_ctx_impl (p q : nat -> bool) ctx : 
-  (forall i, p i -> q i) -> 
-  all_free_vars_ctx p ctx -> all_free_vars_ctx q ctx.
-Proof.
-  intros hpi.
-  eapply alli_impl => i x.
-  apply all_free_vars_decl_impl.
-  intros k; rewrite /shiftnP.
-  now nat_compare_specs.
-Qed.
-
-Lemma closed_decl_all_free_vars {n d} : closed_decl n d -> all_free_vars_decl (closedP n xpredT) d.
-Proof.
-  rewrite /closed_decl /all_free_vars_decl /test_decl.
-  rewrite andb_comm => /andP [cld clb].
-  rewrite (closedP_all_free_vars cld) /=.
-  destruct (decl_body d) eqn:db => /= //.
-  rewrite /foroptb /=.
-  now rewrite (closedP_all_free_vars clb).
-Qed.
-
-Lemma closedn_ctx_all_free_vars {n ctx} : closedn_ctx n ctx ->
-  all_free_vars_ctx (closedP n xpredT) ctx.
-Proof.
-  rewrite /closedn_ctx /all_free_vars_ctx.
-  apply alli_impl => i x.
-  rewrite shiftnP_closedP Nat.add_comm shiftnP_xpredT.
-  eapply closed_decl_all_free_vars.
-Qed.
-
-(** This uses absurdity elimination as [ctx] can't have any free variable *)
-Lemma closed_ctx_all_free_vars P ctx : closed_ctx ctx ->
-  all_free_vars_ctx P ctx.
-Proof.
-  move/closedn_ctx_all_free_vars => /=.
-  rewrite /closedP /=.
-  eapply all_free_vars_ctx_impl => //.
-Qed.
-
-Definition nocc_betweenp k n i :=
-  (i <? k) || (k + n <=? i).
-
-Definition nocc_between k n t := 
-  (all_free_vars (nocc_betweenp k n) t).
-
-Definition noccur_shift p k := fun i => (i <? k) || p (i - k).
-
-Hint Resolve All_forallb_eq_forallb : all.
-
-Definition strengthenP k n (p : nat -> bool) := 
-  fun i => if i <? k then p i else 
-    if i <? k + n then false 
-    else p (i - n).
-
-Instance strengthenP_proper n k : Proper (`=1` ==> `=1`) (strengthenP n k).
-Proof.
-  intros f g Hfg i. rewrite /strengthenP. now rewrite (Hfg i) (Hfg (i - k)).
-Qed.
-
-Lemma shiftnP_strengthenP k' k n p : 
-  shiftnP k' (strengthenP k n p) =1 strengthenP (k' + k) n (shiftnP k' p).
-Proof.
-  intros i. rewrite /shiftnP /strengthenP.
-  repeat nat_compare_specs => /= //. 
-  lia_f_equal.
-Qed.
-
-Lemma all_free_vars_lift (p : nat -> bool) n k t : 
-  all_free_vars (strengthenP k n p) (lift n k t) = all_free_vars p t.
-Proof.
-  intros. revert t n k p.
-  induction t using PCUICInduction.term_forall_list_ind; simpl => //; intros;
-    rewrite ?forallb_map; try eapply All_forallb_eq_forallb; tea; simpl.
-  2-6:try now rewrite ?shiftnP_strengthenP ?IHt1 ?IHt2 ?IHt3.
-  - rename n0 into i. rewrite /strengthenP.
-    repeat nat_compare_specs => //.
-    lia_f_equal.
-  - intros. destruct X. red in X0.
-    rewrite !shiftnP_strengthenP e IHt.
-    f_equal.
-    + solve_all.
-    + f_equal; f_equal.
-      eapply All_forallb_eq_forallb; tea. simpl; intros.
-      now rewrite shiftnP_strengthenP.
-  - unfold test_def in *. simpl; intros ? [].
-    len; rewrite shiftnP_strengthenP. f_equal; eauto.
-  - unfold test_def in *. simpl; intros ? [].
-    len; rewrite shiftnP_strengthenP. f_equal; eauto.
-Qed.
-
-Definition all_free_vars_terms p s :=
-  forallb (all_free_vars p) s.
-  
-Definition substP (k : nat) n (q p : nat -> bool) : nat -> bool :=
-  fun i => 
-    if i <? k then p i
-    else p (i + n) || strengthenP 0 k q i.
-
-Lemma shiftnP_substP k' k n q p : 
-  shiftnP k' (substP k n q p) =1 substP (k' + k) n q (shiftnP k' p).
-Proof.
-  intros i; rewrite /shiftnP /substP.
-  repeat nat_compare_specs => //.
-  f_equal; [f_equal|].
-  * lia_f_equal.
-  * rewrite /strengthenP. simpl.
-    repeat nat_compare_specs => //.
-    lia_f_equal.
-Qed.
-
-Lemma all_free_vars_subst_gen (p q : nat -> bool) s k t : 
-  all_free_vars_terms q s ->
-  all_free_vars p t ->
-  all_free_vars (substP k #|s| q p) (subst s k t).
-Proof.
-  revert t p k.
-  induction t using PCUICInduction.term_forall_list_ind; simpl => //; intros;
-    simpl.
-  all:try (rtoProp; rewrite ?shiftnP_substP; now rewrite ?IHt1 ?IHt2 ?IHt3). 
-  - intros. destruct (Nat.leb_spec k n).
-    * destruct nth_error eqn:eq.
-      + unfold all_free_vars_terms in *. toAll.
-        pose proof (nth_error_Some_length eq).
-        eapply nth_error_all in eq; eauto.
-        simpl in eq. rewrite /substP.
-        eapply all_free_vars_impl. 
-        2:now rewrite -> all_free_vars_lift.
-        rewrite /strengthenP. simpl.
-        intros i. nat_compare_specs => //.
-        intros ->. now rewrite orb_true_r.
-      + eapply nth_error_None in eq.
-        simpl. rewrite /substP.
-        replace (n - #|s| + #|s|) with n by lia.
-        nat_compare_specs.
-        now rewrite H0.
-    * simpl. rewrite /substP /strengthenP /=.
-      rewrite H0. now nat_compare_specs.
-  - solve_all.
-  - rtoProp. destruct X. solve_all.
-    * rewrite shiftnP_substP. solve_all.
-    * rewrite shiftnP_substP; solve_all.
-  - unfold test_def in *; red in X; solve_all.
-    rtoProp. rewrite shiftnP_substP; len. solve_all.
-  - unfold test_def in *; solve_all. rtoProp.
-    rewrite shiftnP_substP; len. solve_all.
-Qed.
-
-Lemma rshiftk_S x f : S (rshiftk x f) = rshiftk (S x) f.
-Proof. reflexivity. Qed.
-
 Lemma red1_rename :
   forall P Σ Γ Δ u v f,
     wf Σ ->
     urenaming P Δ Γ f ->
-    all_free_vars P u ->
+    on_free_vars P u ->
     red1 Σ Γ u v ->
     red1 Σ Δ (rename f u) (rename f v).
 Proof.
@@ -1621,935 +1193,13 @@ Proof.
       now eapply urenaming_context.
     * now len.
 Qed.
- 
-Lemma substP_shiftnP n p : 
-  substP 0 n p (shiftnP n p) =1 p.
-Proof.
-  intros i; rewrite /shiftnP /substP /= /strengthenP /=.
-  nat_compare_specs.
-  replace (i + n - n) with i by lia.
-  now rewrite Nat.sub_0_r orb_diag.
-Qed.
-
-Lemma all_free_vars_subst (p : nat -> bool) s t : 
-  forallb (all_free_vars p) s ->
-  all_free_vars (shiftnP #|s| p) t ->
-  all_free_vars p (subst s 0 t).
-Proof.
-  intros hs ht.
-  epose proof (all_free_vars_subst_gen (shiftnP #|s| p) p s 0 t).
-  rewrite -> substP_shiftnP in H.
-  apply H.
-  - exact hs.
-  - apply ht.
-Qed.
-
-Lemma all_free_vars_subst1 (p : nat -> bool) s t : 
-  all_free_vars p s ->
-  all_free_vars (shiftnP 1 p) t ->
-  all_free_vars p (subst1 s 0 t).
-Proof.
-  intros hs ht.
-  rewrite /subst1.
-  epose proof (all_free_vars_subst_gen (shiftnP 1 p) p [s] 0 t).
-  rewrite -> substP_shiftnP in H.
-  apply H.
-  - now rewrite /all_free_vars_terms /= hs.
-  - apply ht.
-Qed.
-
-Definition addnP n (p : nat -> bool) :=
-  fun i => p (i + n).
-
-Instance addnP_proper n : Proper (`=1` ==> Logic.eq ==> Logic.eq) (addnP n).
-Proof.
-  intros i f g Hfg; now rewrite /addnP.
-Qed.
-  
-Instance addnP_proper_pointwise : Proper (Logic.eq ==> `=1` ==> `=1`) addnP.
-Proof.
-  intros i f g Hfg; now rewrite /addnP.
-Qed.
-
-Lemma addnP_shiftnP n P : addnP n (shiftnP n P) =1 P.
-Proof.
-  intros i; rewrite /addnP /shiftnP /=.
-  nat_compare_specs. lia_f_equal.
-Qed.
-
-Definition on_ctx_free_vars P ctx :=
-  alli (fun k d => P k ==> (all_free_vars_decl (addnP (S k) P) d)) 0 ctx.
-
-Instance on_ctx_free_vars_proper : Proper (`=1` ==> eq ==> eq) on_ctx_free_vars.
-Proof.
-  rewrite /on_ctx_free_vars => f g Hfg x y <-.
-  apply alli_ext => k.
-  now setoid_rewrite Hfg. 
-Qed.
-
-Instance on_ctx_free_vars_proper_pointwise : Proper (`=1` ==> `=1`) on_ctx_free_vars.
-Proof.
-  rewrite /on_ctx_free_vars => f g Hfg x.
-  apply alli_ext => k.
-  now setoid_rewrite Hfg. 
-Qed.
-
-Lemma alli_Alli {A} (p : nat -> A -> bool) n l : 
-  alli p n l <~> Alli p n l.
-Proof.
-  destruct (allbiP p p n l).
-  - intros. destruct (p i x); now constructor.
-  - split; eauto.
-  - split; eauto. by [].
-Qed.
-
-Lemma addnP_add n k p : addnP n (addnP k p) =1 addnP (n + k) p.
-Proof.
-  rewrite /addnP => i. lia_f_equal.
-Qed.
-
-Lemma nth_error_all_free_vars_ctx P n ctx i d :
-  on_ctx_free_vars (addnP n P) ctx ->
-  P (n + i) ->
-  nth_error ctx i = Some d ->
-  test_decl (all_free_vars (addnP (n + S i) P)) d.
-Proof.
-  rewrite /on_ctx_free_vars.
-  solve_all.
-  eapply alli_Alli, Alli_nth_error in H; eauto.
-  rewrite /= {1}/addnP Nat.add_comm H0 /= in H.
-  now rewrite Nat.add_comm -addnP_add.
-Qed.
-
-Definition aboveP k (p : nat -> bool) :=
-  fun i => if i <? k then false else p i.
-
-Lemma strengthenP_addn i p : strengthenP 0 i (addnP i p) =1 aboveP i p.
-Proof.
-   intros k.
-   rewrite /strengthenP /= /addnP /aboveP.
-   nat_compare_specs => //.
-   lia_f_equal.
-Qed.
-
-Lemma all_free_vars_lift0 i p t :
-  all_free_vars (addnP i p) t ->
-  all_free_vars p (lift0 i t).
-Proof.
-  rewrite -(all_free_vars_lift _ i 0).
-  rewrite /strengthenP /= /aboveP /addnP.
-  unshelve eapply all_free_vars_impl.
-  simpl. intros i'. nat_compare_specs => //.
-  now replace (i' - i + i) with i' by lia.
-Qed.
-
-Lemma all_free_vars_lift0_above i p t :
-  all_free_vars (addnP i p) t = all_free_vars (aboveP i p) (lift0 i t).
-Proof.
-  rewrite -(all_free_vars_lift _ i 0).
-  rewrite /strengthenP /= /aboveP /addnP.
-  unshelve eapply all_free_vars_ext.
-  simpl. intros i'. nat_compare_specs => //.
-  now replace (i' - i + i) with i' by lia.
-Qed.
-
-Lemma all_free_vars_mkApps p f args : 
-  all_free_vars p (mkApps f args) = all_free_vars p f && forallb (all_free_vars p) args.
-Proof.
-  induction args in f |- * => /=.
-  - now rewrite andb_true_r.
-  - now rewrite IHargs /= andb_assoc.
-Qed.
-
-Lemma forallb_ext {A} (p q : A -> bool) : p =1 q -> forallb p =1 forallb q.
-Proof.
-  intros hpq l.
-  induction l; simpl; auto.
-  now rewrite (hpq a) IHl.
-Qed.
-
-Instance forallb_proper {A} : Proper (`=1` ==> eq ==> eq) (@forallb A).
-Proof.
-  intros f g Hfg ? ? ->. now apply forallb_ext.
-Qed.
-
-Lemma extended_subst_shiftn p ctx n k : 
-  forallb (all_free_vars (strengthenP 0 n (shiftnP (k + context_assumptions ctx) p))) 
-    (extended_subst ctx (n + k)) =
-  forallb (all_free_vars (shiftnP (k + (context_assumptions ctx)) p)) 
-    (extended_subst ctx k).
-Proof.
-  rewrite lift_extended_subst' forallb_map.
-  eapply forallb_ext => t.
-  rewrite -(all_free_vars_lift _ n 0 t) //.
-Qed.
-
-Lemma extended_subst_shiftn_aboveP p ctx n k : 
-  forallb (all_free_vars (aboveP n p)) (extended_subst ctx (n + k)) =
-  forallb (all_free_vars (addnP n p)) (extended_subst ctx k).
-Proof.
-  rewrite lift_extended_subst' forallb_map.
-  eapply forallb_ext => t.
-  rewrite -(all_free_vars_lift0_above) //.
-Qed.
-
-Lemma extended_subst_shiftn_impl p ctx n k : 
-  forallb (all_free_vars (shiftnP (k + (context_assumptions ctx)) p)) 
-    (extended_subst ctx k) ->
-  forallb (all_free_vars (shiftnP (n + k + context_assumptions ctx) p))
-    (extended_subst ctx (n + k)).
-Proof.
-  rewrite lift_extended_subst' forallb_map.
-  eapply forallb_impl => t _.
-  rewrite -(all_free_vars_lift _ n 0 t).
-  rewrite /strengthenP /=.
-  apply all_free_vars_impl => i.
-  rewrite /shiftnP.
-  repeat nat_compare_specs => //.
-  intros.
-  red; rewrite -H2. lia_f_equal.
-Qed.
-
-Definition occ_betweenP k n :=
-  fun i => (k <=? i) && (i <? k + n).
-
-Lemma shiftn_above_strengthen n k p :
-  forall i,  
-  strengthenP n k p i -> 
-  shiftnP k (aboveP n p) i.
-Proof.
-  intros i. rewrite /shiftnP /aboveP /strengthenP.
-  repeat nat_compare_specs => /= //.
-Abort.
-
-Lemma alli_shiftn {A} n k p (l : list A) :
-    alli p (n + k) l = alli (fun i => p (n + i)) k l.
-Proof.
-  induction l in n, k, p |- *; simpl; auto. f_equal.
-  rewrite (IHl (S n) k p) (IHl 1 k _).
-  apply alli_ext => x.
-  now rewrite Nat.add_succ_r.
-Qed.
-
-
-Lemma addnP0 p : addnP 0 p =1 p.
-Proof. intros i; now rewrite /addnP Nat.add_0_r. Qed.
-
-
-Lemma all_free_vars_decl_all_term P d s :
-  all_free_vars_decl P d = all_free_vars P (mkProd_or_LetIn d (tSort s)).
-Proof.
-  rewrite /all_free_vars_decl /= /test_decl.
-  destruct d as [na [b|] ty] => /= //. rewrite /foroptb /= ?andb_true_r; bool_congr.
-Qed.
-
-Lemma all_free_vars_mkProd_or_LetIn P d t :
-  all_free_vars P (mkProd_or_LetIn d t) = 
-  all_free_vars_decl P d && all_free_vars (shiftnP 1 P) t.
-Proof.
-  destruct d as [na [b|] ty]; rewrite /mkProd_or_LetIn /all_free_vars_decl /test_decl /=
-    ?andb_assoc /foroptb /=; try bool_congr.
-  f_equal. bool_congr.
-Qed.
-
-Lemma all_free_vars_ctx_all_term P ctx s :
-  all_free_vars_ctx P ctx = all_free_vars P (it_mkProd_or_LetIn ctx (tSort s)).
-Proof.
-  rewrite /all_free_vars_ctx.
-  rewrite -{2}[P](shiftnP0 P).
-  generalize 0 as k.
-  induction ctx using rev_ind; simpl; auto; intros k.
-  rewrite List.rev_app_distr alli_app /= andb_true_r.
-  rewrite IHctx it_mkProd_or_LetIn_app /= all_free_vars_mkProd_or_LetIn.
-  now rewrite shiftnP_add.
-Qed.
-
-Lemma expand_lets_it_mkProd_or_LetIn Γ Δ k t : 
-  expand_lets_k Γ k (it_mkProd_or_LetIn Δ t) = 
-  it_mkProd_or_LetIn (expand_lets_k_ctx Γ k Δ) (expand_lets_k Γ (k + #|Δ|) t).
-Proof.
-  revert k; induction Δ as [|[na [b|] ty] Δ] using ctx_length_rev_ind; simpl; auto; intros k.
-  - now rewrite /expand_lets_k_ctx /= Nat.add_0_r.
-  - rewrite it_mkProd_or_LetIn_app /= /mkProd_or_LetIn /=.
-    rewrite /expand_lets_ctx expand_lets_k_ctx_decl /= it_mkProd_or_LetIn_app.
-    simpl. f_equal. rewrite app_length /=.
-    simpl. rewrite Nat.add_1_r Nat.add_succ_r.
-    now rewrite -(H Δ ltac:(lia) (S k)).
-  - rewrite it_mkProd_or_LetIn_app /= /mkProd_or_LetIn /=.
-    rewrite /expand_lets_ctx expand_lets_k_ctx_decl /= it_mkProd_or_LetIn_app.
-    simpl. f_equal. rewrite app_length /=.
-    simpl. rewrite Nat.add_1_r Nat.add_succ_r.
-    now rewrite -(H Δ ltac:(lia) (S k)).
-Qed.
-
-Lemma expand_lets_k_mkApps Γ k f args : 
-  expand_lets_k Γ k (mkApps f args) =
-  mkApps (expand_lets_k Γ k f) (map (expand_lets_k Γ k) args).
-Proof.
-  now rewrite /expand_lets_k lift_mkApps subst_mkApps map_map_compose.
-Qed.
-
-Lemma expand_lets_mkApps Γ f args : 
-  expand_lets Γ (mkApps f args) =
-  mkApps (expand_lets Γ f) (map (expand_lets Γ) args).
-Proof.
-  now rewrite /expand_lets expand_lets_k_mkApps.
-Qed.
-
-Lemma expand_lets_tRel k Γ : 
-  expand_lets Γ (tRel (k + #|Γ|)) = tRel (k + context_assumptions Γ).
-Proof.
-  rewrite /expand_lets /expand_lets_k. 
-  rewrite lift_rel_ge; try lia.
-  rewrite subst_rel_gt; len; try lia.
-  lia_f_equal.
-Qed.
-
-Definition all_free_vars_ctx_k P n ctx :=
-  alli (fun k => (all_free_vars_decl (shiftnP k P))) n (List.rev ctx).
-
-Instance orP_Proper : Proper (`=1` ==> `=1` ==> `=1`) orP.
-Proof.
-  intros f g Hfg f' g' Hfg' i; rewrite /orP.
-  now rewrite Hfg Hfg'.
-Qed.
-
-Instance andP_Proper : Proper (`=1` ==> `=1` ==> `=1`) conjP.
-Proof.
-  intros f g Hfg f' g' Hfg' i; rewrite /conjP.
-  now rewrite Hfg Hfg'.
-Qed.
-
-Instance implP_Proper : Proper (`=1` ==> `=1` ==> `=1`) implP.
-Proof.
-  intros f g Hfg f' g' Hfg' i; rewrite /implP.
-  now rewrite Hfg Hfg'.
-Qed.
-
-Lemma orPL (p q : nat -> bool) : implP p (orP p q) =1 xpredT.
-Proof.
-  intros i. rewrite /implP /orP.
-  rewrite (ssrbool.implybE (p i)).
-  destruct (p i) => //.
-Qed.
-
-Lemma orPR (p q : nat -> bool) i : q i -> (orP p q) i.
-Proof.
-  rewrite /orP => ->; rewrite orb_true_r //.
-Qed.
-
-Lemma all_free_vars_implP p q t : 
-  implP p q =1 xpredT ->
-  all_free_vars p t -> all_free_vars q t.
-Proof.
-  rewrite /implP. intros Hp.
-  eapply all_free_vars_impl.
-  intros i hp. specialize (Hp i). now rewrite hp in Hp.
-Qed.
-
-Definition shiftnP_orP n p q : 
-  shiftnP n (orP p q) =1 orP (shiftnP n p) (shiftnP n q).
-Proof.
-  intros i.
-  rewrite /shiftnP /orP.
-  repeat nat_compare_specs => //.
-Qed.
-
-Lemma addnP_orP n p q : addnP n (orP p q) =1 orP (addnP n p) (addnP n q).
-Proof. reflexivity. Qed.
-
-(** We need a disjunction here as the substitution can be made of 
-    expanded lets (properly lifted) or just the variables of 
-    [ctx] (lifted by [k]).
-    
-    The proof could certainly be simplified using a more high-level handling of
-    free-variables predicate, which form a simple classical algebra. 
-    To investigate: does ssr's library support this? *)
-
-Lemma all_free_vars_extended_subst p k ctx :
-  all_free_vars_ctx_k p k ctx ->
-  forallb (all_free_vars 
-    (orP (strengthenP 0 (context_assumptions ctx + k) (shiftnP k p)) 
-      (occ_betweenP k (context_assumptions ctx))))
-    (extended_subst ctx k).
-Proof.
-  rewrite /all_free_vars_ctx_k.
-  induction ctx as [|[na [b|] ty] ctx] in p, k |- *; auto.
-  - simpl. rewrite alli_app /= andb_true_r=> /andP [] hctx.
-    rewrite /all_free_vars_decl /test_decl /=; len => /andP [] hty /= hb.
-    specialize (IHctx _ k hctx).
-    rewrite IHctx // andb_true_r.
-    eapply all_free_vars_subst => //.
-    len. erewrite all_free_vars_implP => //; cycle 1.
-    { erewrite all_free_vars_lift; eauto. }
-    rewrite shiftnP_orP.
-    now rewrite shiftnP_strengthenP Nat.add_0_r shiftnP_add orPL.
-  - cbn. rewrite alli_app /= andb_true_r => /andP [] hctx.
-    rewrite /all_free_vars_decl /test_decl andb_true_r /= => hty.
-    len in hty.
-    specialize (IHctx p k).
-    rewrite orPR /=.
-    * rewrite /occ_betweenP. repeat nat_compare_specs => /= //.
-    * specialize (IHctx hctx).
-      rewrite (lift_extended_subst' _ 1).
-      rewrite forallb_map.
-      solve_all.
-      apply all_free_vars_lift0.
-      rewrite addnP_orP.
-      eapply all_free_vars_implP; eauto.
-      intros i. unfold implP, orP.
-      rewrite /strengthenP /= /addnP /=.
-      repeat nat_compare_specs => /= //.
-      + rewrite /occ_betweenP /implP => /=.
-        repeat nat_compare_specs => /= //.
-      + rewrite /shiftnP /occ_betweenP /=.
-        repeat nat_compare_specs => /= //.
-        rewrite !orb_false_r.
-        replace (i + 1 - S (context_assumptions ctx + k) - k) with
-          (i - (context_assumptions ctx + k) - k) by lia.
-        rewrite implybE. destruct p; auto. 
-Qed.
-
-Lemma all_free_vars_expand_lets_k P Γ n t : 
-  n = context_assumptions Γ ->
-  all_free_vars_ctx P Γ ->
-  all_free_vars (shiftnP #|Γ| P) t ->
-  all_free_vars (shiftnP n P) (expand_lets_k Γ 0 t).
-Proof.
-  intros -> HΓ Ht.
-  rewrite /expand_lets_k /=.
-  eapply all_free_vars_impl; cycle 1.
-  - eapply all_free_vars_subst_gen.
-    1:eapply all_free_vars_extended_subst; eauto.
-    rewrite -> all_free_vars_lift. eauto.
-  - len. rewrite /substP /= /strengthenP /=.
-    intros i. simpl. rewrite /shiftnP.
-    repeat nat_compare_specs => /= //.
-    rewrite Nat.sub_0_r. rewrite /orP.
-    replace (i + #|Γ| - context_assumptions Γ - #|Γ|) with (i - context_assumptions Γ) by lia.
-    rewrite /occ_betweenP. repeat nat_compare_specs => /= //.
-    rewrite orb_false_r Nat.sub_0_r.
-    now rewrite orb_diag.
-Qed.
-
-Lemma all_free_vars_terms_inds P ind puinst bodies : 
-  all_free_vars_terms P (inds ind puinst bodies).
-Proof.
-  rewrite /inds.
-  induction #|bodies|; simpl; auto.
-Qed.
-
-Lemma all_free_vars_decl_map P f d :
-  (forall i, all_free_vars P i = all_free_vars P (f i)) ->
-  all_free_vars_decl P d = all_free_vars_decl P (map_decl f d).
-Proof.
-  intros Hi.
-  rewrite /all_free_vars_decl /test_decl.
-  rewrite Hi. f_equal.
-  simpl. destruct (decl_body d) => //.
-  now rewrite /foroptb /= (Hi t).
-Qed.
-
-Lemma all_free_vars_subst_instance_context P u Γ :
-  all_free_vars_ctx P (subst_instance_context u Γ) = all_free_vars_ctx P Γ.
-Proof.
-  rewrite /all_free_vars_ctx.
-  rewrite /subst_instance_context -map_rev alli_map.
-  apply alli_ext => i d.
-  symmetry. apply all_free_vars_decl_map.
-  intros. apply all_free_vars_subst_instance.
-Qed.
-
-Lemma all_free_vars_map2_cstr_args p bctx ctx :
-  #|bctx| = #|ctx| ->
-  all_free_vars_ctx p ctx =
-  all_free_vars_ctx p (map2 set_binder_name bctx ctx).
-Proof.
-  rewrite /all_free_vars_ctx.
-  induction ctx as [|d ctx] in bctx |- *; simpl; auto.
-  - destruct bctx; reflexivity.
-  - destruct bctx => /= //.
-    intros [= hlen].
-    rewrite alli_app (IHctx bctx) // alli_app. f_equal.
-    len. rewrite map2_length // hlen. f_equal.
-Qed.
-
-Lemma all_free_vars_case_branch_context {Σ} {wfΣ : wf Σ} {P ci i mdecl idecl p br cdecl} :
-  let brctx := case_branch_context ci mdecl p (bcontext br) cdecl in
-  declared_constructor Σ (ci, i) mdecl idecl cdecl ->
-  wf_predicate mdecl idecl p ->
-  wf_branch cdecl br ->
-  forallb (all_free_vars P) (pparams p) ->
-  all_free_vars_ctx P brctx.
-Proof.
-  intros brctx decli wfp wfb havp.
-  rewrite /brctx /case_branch_context /case_branch_context_gen.
-  rewrite (all_free_vars_ctx_all_term _ _ Universe.type0).
-  rewrite -(subst_it_mkProd_or_LetIn _ _ _ (tSort _)).
-  apply all_free_vars_subst => //.
-  rewrite -(expand_lets_it_mkProd_or_LetIn _ _ 0 (tSort _)).
-  eapply all_free_vars_expand_lets_k; len.
-  * rewrite (wf_predicate_length_pars wfp).
-    apply (declared_minductive_ind_npars decli).
-  * eapply closed_ctx_all_free_vars.
-    rewrite closedn_subst_instance_context.
-    apply (declared_inductive_closed_params decli).
-  * rewrite -(subst_it_mkProd_or_LetIn _ _ _ (tSort _)).
-    eapply all_free_vars_impl; cycle 1.
-    + eapply (all_free_vars_subst_gen _ P).
-      { eapply all_free_vars_terms_inds. }
-      rewrite -all_free_vars_ctx_all_term.
-      rewrite all_free_vars_subst_instance_context.
-      rewrite -all_free_vars_map2_cstr_args.
-      { apply (wf_branch_length wfb). }
-      instantiate (1 := closedP (#|mdecl.(ind_bodies)| + #|mdecl.(ind_params)|) xpredT).
-      eapply closedn_ctx_all_free_vars.
-      now move/andP: (declared_constructor_closed wfΣ decli) => [] /andP [].
-    + intros i'.
-      rewrite /substP /= /closedP /shiftnP. len.
-      now repeat nat_compare_specs => /= //.
-Qed.
-
-Lemma all_free_vars_to_extended_list P ctx : 
-  forallb (all_free_vars (shiftnP #|ctx| P)) (to_extended_list ctx).
-Proof.
-  rewrite /to_extended_list /to_extended_list_k.
-  change #|ctx| with (0 + #|ctx|).
-  have: (forallb (all_free_vars (shiftnP (0 + #|ctx|) P)) []) by easy.
-  generalize (@nil term), 0.
-  induction ctx; intros l n.
-  - simpl; auto.
-  - simpl. intros Hl.
-    destruct a as [? [?|] ?].
-    * rewrite Nat.add_succ_r in Hl.
-      specialize (IHctx _ (S n) Hl).
-      now rewrite Nat.add_succ_r Nat.add_1_r.
-    * rewrite Nat.add_succ_r Nat.add_1_r. eapply (IHctx _ (S n)).
-      rewrite -[_ + _](Nat.add_succ_r n #|ctx|) /= Hl.
-      rewrite /shiftnP.
-      nat_compare_specs => /= //.
-Qed.
-
-(** This is less precise than the strengthenP lemma above *)
-Lemma all_free_vars_lift_impl (p : nat -> bool) (n k : nat) (t : term) :
-  all_free_vars (shiftnP k p) t ->
-  all_free_vars (shiftnP (n + k) p) (lift n k t).
-Proof.
-  rewrite -(all_free_vars_lift _ n k t).
-  eapply all_free_vars_impl.
-  intros i.
-  rewrite /shiftnP /strengthenP.
-  repeat nat_compare_specs => /= //.
-  now replace (i - n - k) with (i - (n + k)) by lia.
-Qed.
-
-Lemma all_free_vars_case_predicate_context {Σ} {wfΣ : wf Σ} {P ci mdecl idecl p} :
-  let pctx := case_predicate_context ci mdecl idecl p in
-  declared_inductive Σ ci mdecl idecl ->
-  wf_predicate mdecl idecl p ->
-  forallb (all_free_vars P) (pparams p) ->
-  all_free_vars (shiftnP #|pcontext p| P) (preturn p) ->
-  all_free_vars_ctx P pctx.
-Proof.
-  intros pctx decli wfp wfb havp.
-  rewrite /pctx /case_predicate_context /case_predicate_context_gen.
-  set (ibinder := {| decl_name := _ |}).
-  rewrite -all_free_vars_map2_cstr_args /=; len.
-  { eapply (wf_predicate_length_pcontext wfp). }
-  rewrite alli_app; len; rewrite andb_true_r.
-  apply andb_true_iff. split.
-  - rewrite -/(all_free_vars_ctx P _).
-    rewrite (all_free_vars_ctx_all_term _ _ Universe.type0).
-    rewrite -(subst_it_mkProd_or_LetIn _ _ _ (tSort _)).
-    apply all_free_vars_subst => //.
-    rewrite -all_free_vars_ctx_all_term.
-    rewrite all_free_vars_subst_instance_context.
-    rewrite (all_free_vars_ctx_all_term _ _ (Universe.type0)).
-    rewrite -(expand_lets_it_mkProd_or_LetIn _ _ 0 (tSort _)).
-    eapply all_free_vars_expand_lets_k; len.
-    * rewrite (wf_predicate_length_pars wfp).
-      apply (declared_minductive_ind_npars decli).
-    * eapply closed_ctx_all_free_vars.
-      apply (declared_inductive_closed_params decli).
-    * eapply all_free_vars_impl; cycle 1.
-      { rewrite <- all_free_vars_ctx_all_term.
-        instantiate (1 := closedP #|mdecl.(ind_params)| xpredT).
-        eapply closedn_ctx_all_free_vars.
-        move: (declared_inductive_closed_pars_indices wfΣ decli).
-        now rewrite closedn_ctx_app => /andP []. }
-       intros i'.
-      rewrite /substP /= /closedP /shiftnP. len.
-      now repeat nat_compare_specs => /= //.
-  - rewrite /all_free_vars_decl /ibinder /test_decl /= /foroptb /= andb_true_r.
-    rewrite all_free_vars_mkApps /= forallb_app /=.
-    rewrite all_free_vars_to_extended_list /= andb_true_r.
-    rewrite -/(is_true _).
-    rewrite forallb_map. unshelve eapply (forallb_impl _ _ _ _ wfb).
-    intros. simpl.
-    eapply all_free_vars_lift0. now rewrite addnP_shiftnP.
-Qed.
-
-Lemma forall_free_vars_extended_subst brctx p :
-  all_free_vars_ctx p brctx ->
-  forallb (all_free_vars (shiftnP (context_assumptions brctx) p))
-    (extended_subst brctx 0).
-Proof.
-  move/all_free_vars_extended_subst.
-  eapply forallb_impl.
-  intros x hin.
-  rewrite Nat.add_0_r shiftnP0.
-  eapply all_free_vars_impl.
-  intros i. rewrite /orP /strengthenP /= /occ_betweenP /shiftnP.
-  repeat nat_compare_specs => /= //.
-  now rewrite orb_false_r.
-Qed.
-
-Lemma all_free_vars_fix_subst P mfix idx :
-  all_free_vars P (tFix mfix idx) ->
-  forallb (all_free_vars P) (fix_subst mfix).
-Proof.
-  move=> /=; rewrite /fix_subst.
-  intros hmfix. generalize hmfix.
-  induction mfix at 2 4; simpl; auto.
-  move/andP => [ha hm]. rewrite IHm // andb_true_r //.
-Qed.
-
-Lemma all_free_vars_unfold_fix P mfix idx narg fn :
-  unfold_fix mfix idx = Some (narg, fn) ->
-  all_free_vars P (tFix mfix idx) ->
-  all_free_vars P fn.
-Proof.
-  rewrite /unfold_fix. 
-  destruct nth_error eqn:hnth => // [=] _ <- /=.
-  intros hmfix; generalize hmfix.
-  move/forallb_All/(nth_error_all hnth) => /andP [] _ Hbody.
-  eapply all_free_vars_subst; len => //.
-  eapply (all_free_vars_fix_subst _ _ idx) => //.
-Qed.
-
-Lemma all_free_vars_cofix_subst P mfix idx :
-  all_free_vars P (tCoFix mfix idx) ->
-  forallb (all_free_vars P) (cofix_subst mfix).
-Proof.
-  move=> /=; rewrite /cofix_subst.
-  intros hmfix. generalize hmfix.
-  induction mfix at 2 4; simpl; auto.
-  move/andP => [ha hm]. rewrite IHm // andb_true_r //.
-Qed.
-
-Lemma all_free_vars_unfold_cofix P mfix idx narg fn :
-  unfold_cofix mfix idx = Some (narg, fn) ->
-  all_free_vars P (tCoFix mfix idx) ->
-  all_free_vars P fn.
-Proof.
-  rewrite /unfold_cofix. 
-  destruct nth_error eqn:hnth => // [=] _ <- /=.
-  intros hmfix; generalize hmfix.
-  move/forallb_All/(nth_error_all hnth) => /andP [] _ Hbody.
-  eapply all_free_vars_subst; len => //.
-  eapply (all_free_vars_cofix_subst _ _ idx) => //.
-Qed.
-
-Lemma nth_error_forallb {A} {p : A -> bool} {l : list A} {n x} :
-  nth_error l n = Some x -> forallb p l -> p x.
-Proof.
-  intros Hnth HPl. 
-  induction l in n, Hnth, HPl |- * => //.
-  - rewrite nth_error_nil in Hnth => //.
-  - destruct n => /=; noconf Hnth.
-    * now move: HPl => /= /andP.
-    * eapply IHl; tea. now move: HPl => /andP.
-Qed.
-
-Lemma addnP_shiftnP_comm n (P : nat -> bool) : P 0 -> addnP 1 (shiftnP n P) =1 shiftnP n (addnP 1 P).
-Proof.
-  intros p0 i; rewrite /addnP /shiftnP /=.
-  repeat nat_compare_specs => /= //. 
-  - assert (n = i + 1) as -> by lia.
-    now replace (i + 1 - (i + 1)) with 0 by lia.
-  - lia_f_equal.
-Qed.
-
-Lemma on_ctx_free_vars_concat P Γ Δ : 
-  on_ctx_free_vars P Γ ->
-  on_ctx_free_vars (shiftnP #|Δ| P) Δ ->  
-  on_ctx_free_vars (shiftnP #|Δ| P) (Γ ,,, Δ).
-Proof.
-  rewrite /on_ctx_free_vars alli_app.
-  move=> hΓ -> /=; rewrite alli_shiftn.
-  eapply alli_impl; tea => i d /=.
-  simpl.
-  rewrite {1}/shiftnP. nat_compare_specs.
-  replace (#|Δ| + i - #|Δ|) with i by lia.
-  destruct (P i) eqn:pi => /= //.
-  apply all_free_vars_decl_impl => k.
-  rewrite /addnP /shiftnP.
-  nat_compare_specs.
-  now replace (k + S (#|Δ| + i) - #|Δ|) with (k + S i) by lia.
-Qed.
-
-Lemma on_ctx_free_vars_tip P d : on_ctx_free_vars P [d] = P 0 ==> all_free_vars_decl (addnP 1 P) d.
-Proof.
-  now rewrite /on_ctx_free_vars /= /= andb_true_r.
-Qed.
-
-Lemma OnOne2_impl_All_r {A} (P : A -> A -> Type) (Q : A -> Type) l l' : 
-  (forall x y, Q x -> P x y -> Q y) ->
-  OnOne2 P l l' -> All Q l -> All Q l'.
-Proof.
-  intros HPQ.
-  induction 1; intros H; depelim H; constructor; auto.
-  now eapply HPQ.
-Qed.
-
-Lemma OnOne2All_impl_All_r {A B} (P : B -> A -> A -> Type) (Q : A -> Type) i l l' : 
-  (forall i x y, Q x -> P i x y -> Q y) ->
-  OnOne2All P i l l' -> All Q l -> All Q l'.
-Proof.
-  intros HPQ.
-  induction 1; intros H; depelim H; constructor; auto.
-  now eapply HPQ.
-Qed.
-
-Lemma shiftnPS n P : shiftnP (S n) P n.
-Proof.
-  rewrite /shiftnP /=.
-  now nat_compare_specs.
-Qed.
-
-Lemma on_ctx_free_vars_extend P Γ Δ :
-  all_free_vars_ctx P Δ ->
-  on_ctx_free_vars P Γ ->
-  on_ctx_free_vars (shiftnP #|Δ| P) (Γ ,,, Δ).
-Proof.
-  intros hΔ hΓ.
-  apply on_ctx_free_vars_concat => //.
-  revert P Γ hΓ hΔ.
-  induction Δ using rev_ind; simpl; auto; intros P Γ hΓ.
-  rewrite /on_ctx_free_vars /all_free_vars_ctx List.rev_app_distr /= shiftnP0.
-  rewrite alli_shift. setoid_rewrite Nat.add_comm. setoid_rewrite <- shiftnP_add.
-  move/andP=> [] hx hΔ.
-  rewrite alli_app /= andb_true_r Nat.add_0_r; len.
-  rewrite Nat.add_comm.
-  rewrite addnP_shiftnP.
-  specialize (IHΔ (shiftnP 1 P) (Γ ,, x)).
-  forward IHΔ.
-  * simpl. apply (on_ctx_free_vars_concat _ _ [x]) => //.
-    simpl.
-    now rewrite on_ctx_free_vars_tip {1}/shiftnP /= addnP_shiftnP.
-  * specialize (IHΔ hΔ).
-    rewrite shiftnPS /= hx andb_true_r.
-    rewrite /on_ctx_free_vars in IHΔ.
-    rewrite -(Nat.add_1_r #|Δ|).
-    setoid_rewrite <-(shiftnP_add).
-    now setoid_rewrite <- (shiftnP_add _ _ _ _).
-Qed.
-
-Lemma OnOne2All_nth_error {A B} (P : A -> B -> B -> Type) il l l' :
-  OnOne2All P il l l' ->
-  OnOne2All (fun i x y => (∑ ni, nth_error il ni = Some i) * P i x y) il l l'.
-Proof.
-  induction 1.
-  - econstructor => //.
-    split => //.
-    exists 0; reflexivity.
-  - constructor. eapply (OnOne2All_impl IHX).
-    intros i x y [[ni hni] ?].
-    split; auto. exists (S ni). apply hni.
-Qed.
-
-Lemma all_free_vars_fix_context P mfix : 
-  All (fun x : def term =>
-      test_def (all_free_vars P) (all_free_vars (shiftnP #|mfix| P)) x)
-      mfix ->
-  all_free_vars_ctx P (fix_context mfix).
-Proof.
-  intros a.
-  assert (All (fun x => all_free_vars P x.(dtype)) mfix).
-  { solve_all. now move/andP: H=> []. } clear a.
-  induction mfix using rev_ind; simpl; auto.
-  rewrite /fix_context /= mapi_app List.rev_app_distr /=.
-  rewrite /all_free_vars_ctx /= alli_app. len.
-  rewrite andb_true_r.
-  eapply All_app in X as [X Hx].
-  depelim Hx. clear Hx.
-  specialize (IHmfix X).
-  rewrite /all_free_vars_ctx in IHmfix.
-  rewrite IHmfix /= /all_free_vars_decl /test_decl /= /foroptb /= andb_true_r.
-  apply all_free_vars_lift0.
-  now rewrite addnP_shiftnP.
-Qed.
-(* 
-Definition all_free_vars_ctx_gen P ctx :=
-  alli (fun k => (all_free_vars_decl (addnP k P))) 0 ctx.
-
-Instance all_free_vars_ctx_gen_proper : Proper (`=1` ==> `=1`) all_free_vars_ctx_gen.
-Proof.
-  rewrite /all_free_vars_ctx_gen => f g Hfg x.
-  now setoid_rewrite Hfg. 
-Qed.
-
-Lemma all_free_vars_ctx_gen_decl (P : nat -> bool) (Q : nat -> bool) Γ i d : 
-  nth_error Γ i = Some d ->
-  P i ->
-  (forall k, all_free_vars (addnP i Q) k -> all_free_vars (addnP i P) k) ->
-  all_free_vars_ctx_gen Q Γ -> 
-  test_decl (all_free_vars (addnP i P)) d.
-Proof.
-  rewrite /all_free_vars_ctx_gen.
-  solve_all.
-  eapply alli_Alli, Alli_nth_error in H2; eauto.
-  simpl in H1. rewrite /all_free_vars_decl in H1.
-  eapply test_decl_impl. 2:eapply H2.
-  intros. simpl in H3. apply H1. auto.
-Qed. *)
-
-
-(** This shows preservation by reduction of closed/noccur_between predicates 
-  necessary to prove exchange and strengthening lemmas. *)
-Lemma red1_all_free_vars {P : nat -> bool} {Σ Γ u v} {wfΣ : wf Σ} :
-  all_free_vars P u ->
-  (* (forall i k, P i -> (* The ith variable of Γ is present  *)
-  (* k respect Q for the prefix of Γ from begginning to i, i.e. k 
-    is under Γ_i *)
-  all_free_vars (addnP (S i) Q) k -> 
-  (* P holds *)
-  all_free_vars (addnP (S i) P) k) -> *)
-  on_ctx_free_vars P Γ ->
-  red1 Σ Γ u v ->
-  all_free_vars P v.
-Proof.
-  intros hav hctx h.
-  induction h using red1_ind_all in P, hav, hctx |- *.
-  all: try solve [
-    simpl ; constructor ; eapply IHh ;
-    try (simpl in hav; rtoProp);
-    try eapply urenaming_vass ;
-    try eapply urenaming_vdef ;
-    assumption
-  ].
-  all:simpl in hav |- *; try toAll.
-  all:try move/and3P: hav => [h1 h2 h3].
-  all:try (move/andP: hav => [] /andP [] h1 h2 h3).
-  all:try move/andP: hav => [h1 h2].
-  all:try move/andP: h3 => [] h3 h4.
-  all:try rewrite ?h1 // ?h2 // ?h3 // ?h4 // ?IHh /= // ?andb_true_r.
-  all:try eapply all_free_vars_subst1; eauto.
-  - destruct (nth_error Γ i) eqn:hnth => //.
-    simpl in H. noconf H.
-    epose proof (nth_error_all_free_vars_ctx P 0 Γ i c).
-    forward H0. { now rewrite addnP0. }
-    specialize (H0 hav hnth). simpl in H0.
-    rewrite /test_decl H in H0.
-    rewrite all_free_vars_lift0 //.
-    move/andP: H0 => [].
-    now rewrite /foroptb /= => _ hbod.
-  - rewrite /iota_red. rename h4 into hbrs.
-    move: h3. rewrite all_free_vars_mkApps => /andP [] hf hargs.
-    apply all_free_vars_subst.
-    { rewrite forallb_skipn //. }
-    rewrite H2.
-    rewrite /expand_lets /expand_lets_k /=.
-    eapply all_free_vars_subst.
-    * eapply forall_free_vars_extended_subst.
-      eapply all_free_vars_case_branch_context; eauto.
-    * rewrite extended_subst_length.
-      rewrite (case_branch_context_length H1).
-      rewrite shiftnP_add.
-      eapply nth_error_forallb in hbrs; eauto.
-      simpl in hbrs.
-      eapply all_free_vars_lift_impl in hbrs.
-      now rewrite Nat.add_comm.
-  - rewrite !all_free_vars_mkApps in hav |- *.
-    rtoProp.
-    eapply all_free_vars_unfold_fix in H; eauto. 
-  - move: h3; rewrite !all_free_vars_mkApps.
-    move=> /andP[] hcofix ->.
-    eapply all_free_vars_unfold_cofix in hcofix; eauto.
-    now rewrite hcofix.
-  - move: hav; rewrite !all_free_vars_mkApps => /andP [] hcofix ->.
-    eapply all_free_vars_unfold_cofix in H as ->; eauto.
-  - eapply closed_all_free_vars. rewrite closedn_subst_instance_constr.
-    eapply declared_constant_closed_body; eauto.
-  - move: hav; rewrite all_free_vars_mkApps /=.
-    now move/(nth_error_forallb H).
-  - rewrite (on_ctx_free_vars_concat _ _ [_]) // /=
-      on_ctx_free_vars_tip /= addnP_shiftnP /all_free_vars_decl
-      /test_decl /= andb_true_r //.
-  - rewrite (on_ctx_free_vars_concat _ _ [_]) //
-      on_ctx_free_vars_tip /= addnP_shiftnP /all_free_vars_decl /test_decl /= h2 /=
-      /foroptb /= h1 //.
-  - solve_all.
-    eapply OnOne2_impl_All_r; eauto. solve_all.
-  - rewrite /pctx.
-    rewrite -(case_predicate_context_length (ci:=ci) H).
-    eapply on_ctx_free_vars_extend => //.
-    apply (all_free_vars_case_predicate_context isdecl H h1 h2).
-  - toAll.
-    eapply Forall2_All2 in H0.
-    eapply OnOne2All_All2_mix_left in X; eauto.
-    eapply OnOne2All_nth_error in X.
-    eapply OnOne2All_impl_All_r in X; eauto; solve_all.
-    destruct a as [cidx hnth].
-    rewrite -b. eapply b1 => //.
-    erewrite <- (case_branch_context_length b0).
-    eapply on_ctx_free_vars_extend => //.
-    eapply (all_free_vars_case_branch_context (i := cidx)); eauto.
-    * split; eauto.
-    * solve_all.
-  - rewrite (on_ctx_free_vars_concat _ _ [_]) // /=
-      on_ctx_free_vars_tip /= addnP_shiftnP /all_free_vars_decl /test_decl /= h1 /= //.
-  - toAll. eapply OnOne2_impl_All_r; eauto; solve_all.
-  - toAll. unfold test_def.
-    rewrite -(OnOne2_length X).
-    eapply OnOne2_impl_All_r; eauto; solve_all.
-    destruct x, y; noconf b; simpl in *. rtoProp; solve_all.
-  - toAll. unfold test_def in *. rewrite -(OnOne2_length X).
-    eapply OnOne2_impl_All_r; eauto; solve_all.
-    destruct x, y; noconf b; simpl in *; rtoProp; solve_all.
-    apply b0 => //.
-    rewrite -(fix_context_length mfix0).
-    eapply on_ctx_free_vars_extend => //.
-    now apply all_free_vars_fix_context.
-  - toAll. unfold test_def.
-    rewrite -(OnOne2_length X).
-    eapply OnOne2_impl_All_r; eauto; solve_all.
-    destruct x, y; noconf b; simpl in *. rtoProp; solve_all.
-  - toAll. unfold test_def in *. rewrite -(OnOne2_length X).
-    eapply OnOne2_impl_All_r; eauto; solve_all.
-    destruct x, y; noconf b; simpl in *; rtoProp; solve_all.
-    apply b0 => //.
-    rewrite -(fix_context_length mfix0).
-    eapply on_ctx_free_vars_extend => //.
-    now apply all_free_vars_fix_context.
-Qed.
-
-(* Lemma cumul_rename :
-  forall P Σ Γ Δ f A B,
-    wf Σ.1 ->
-    urenaming (shiftnP #|Γ| P) Δ Γ f ->
-    Σ ;;; Γ |- A <= B ->
-    Σ ;;; Δ |- rename f A <= rename f B.
-Proof.
-  intros P Σ Γ Δ f A B hΣ hf h.
-  induction h.
-  - eapply cumul_refl. eapply eq_term_upto_univ_rename. assumption.
-  - eapply cumul_red_l.
-    + eapply red1_rename. all: try eassumption.
-    + apply IHh.
-      * eapply (red1_all_free_vars hA); tea.
-      * auto.
-  - eapply cumul_red_r.
-    + eapply IHh; eauto. eapply (red1_all_free_vars hB); tea.
-    + eapply red1_rename. all: try eassumption.
-Qed. *)
 
 Lemma cumul_renameP :
   forall P Σ Γ Δ f A B,
     wf Σ.1 ->
     urenaming P Δ Γ f ->
-    all_free_vars P A ->
-    all_free_vars P B ->
+    on_free_vars P A ->
+    on_free_vars P B ->
     on_ctx_free_vars P Γ ->
     Σ ;;; Γ |- A <= B ->
     Σ ;;; Δ |- rename f A <= rename f B.
@@ -2560,10 +1210,10 @@ Proof.
   - eapply cumul_red_l.
     + eapply red1_rename. all: try eassumption.
     + apply IHh.
-      * eapply (red1_all_free_vars hA); tea.
+      * eapply (red1_on_free_vars hA); tea.
       * auto.
   - eapply cumul_red_r.
-    + eapply IHh; eauto. eapply (red1_all_free_vars hB); tea.
+    + eapply IHh; eauto. eapply (red1_on_free_vars hB); tea.
     + eapply red1_rename. all: try eassumption.
 Qed.
 
@@ -2639,53 +1289,6 @@ Proof.
       { reflexivity. } now eapply urenaming_context.
 Qed.
 
-Lemma All2i_map {A B C D} (R : nat -> C -> D -> Type) (f : A -> C) (g : B -> D) n l l' :
-  All2i (fun i x y => R i (f x) (g y)) n l l' -> All2i R n (map f l) (map g l').
-Proof. induction 1; simpl; constructor; try congruence. Qed.
-
-Lemma All2i_map_right {B C D} (R : nat -> C -> D -> Type) (g : B -> D) n l l' :
-  All2i (fun i x y => R i x (g y)) n l l' -> All2i R n l (map g l').
-Proof. induction 1; simpl; constructor; try congruence. Qed.
-
-Lemma All2i_nth_impl_gen {A B} (R : nat -> A -> B -> Type) n l l' :
-  All2i R n l l' ->
-  All2i (fun i x y => 
-    (if i <? n then False
-    else nth_error l (i - n) = Some x) * R i x y) n l l'.
-Proof.
-  intros a. depind a.
-  - constructor.
-  - constructor.
-    * simpl. destruct (Nat.ltb n n) eqn:ltb.
-      + eapply Nat.ltb_lt in ltb. lia.
-      + rewrite Nat.sub_diag. auto.
-    * simpl. eapply (All2i_impl IHa).
-      intros. destruct (Nat.ltb i (S n)) eqn:ltb; simpl in *; destruct X =>  //.
-      apply Nat.ltb_nlt in ltb. 
-      destruct (Nat.ltb i n) eqn:ltb'; simpl in *.
-      + eapply Nat.ltb_lt in ltb'. lia.
-      + eapply Nat.ltb_nlt in ltb'.
-        assert (i - n = S (i - S n)) as -> by lia. simpl. now rewrite e.
-Qed.
-
-Lemma All2i_nth_hyp {A B} (R : nat -> A -> B -> Type) l l' :
-  All2i R 0 l l' ->
-  All2i (fun i x y => (nth_error l i = Some x) * R i x y) 0 l l'.
-Proof.
-  intros a.
-  eapply All2i_nth_impl_gen in a. simpl in a.
-  eapply (All2i_impl a). intros.
-  now rewrite Nat.sub_0_r in X.
-Qed.
-
-Lemma case_branch_type_length {ci mdecl idecl p br ptm i cdecl} :
-  wf_branch cdecl br ->
-  #|(case_branch_type ci mdecl idecl p br ptm i cdecl).1| = #|cstr_args cdecl|.
-Proof.
-  intros wf; simpl.
-  now rewrite case_branch_context_length_args.
-Qed.
-
 Lemma rename_decompose_prod_assum f Γ t :
     decompose_prod_assum (rename_context f Γ) (rename (shiftn #|Γ| f) t)
     = let '(Γ, t) := decompose_prod_assum Γ t in (rename_context f Γ, rename (shiftn #|Γ| f) t).
@@ -2706,9 +1309,6 @@ Proof.
   rewrite /rename_context fold_context_app /app_context. f_equal.
   apply fold_context_ext. intros i x. now rewrite shiftn_add.
 Qed.
-
-Lemma fold_context_tip f d : fold_context f [d] = [map_decl (f 0) d].
-Proof. reflexivity. Qed.
 
 Lemma rename_smash_context f Γ Δ :
   rename_context f (smash_context Γ Δ) = 
@@ -2775,22 +1375,6 @@ Proof.
   rewrite rename_mkApps. simpl. rewrite decompose_app_mkApps //.
 Qed.
 
-Lemma map_option_out_impl {A B} (l : list A) (f g : A -> option B) x :
-  (forall x y, f x = Some y -> g x = Some y) ->
-  map_option_out (map f l) = Some x ->
-  map_option_out (map g l) = Some x.
-Proof.
-  intros Hfg.
-  induction l in x |- *; simpl; auto.
-  destruct (f a) eqn:fa.
-  - rewrite (Hfg _ _ fa).
-    move: IHl; destruct map_option_out.
-    * move=> H'. specialize (H' _ eq_refl).
-      rewrite H'. congruence.
-    * discriminate.
-  - discriminate.
-Qed.
-
 Lemma rename_wf_fixpoint Σ f mfix :
   wf_fixpoint Σ mfix ->
   wf_fixpoint Σ (map (map_def (rename f) (rename (shiftn #|mfix| f))) mfix).
@@ -2812,41 +1396,6 @@ Proof.
   eapply map_option_out_impl in hmap.
   2:{ intros x y. apply (rename_check_one_cofix f mfix). }
   now rewrite hmap.
-Qed.
-(*
-Lemma wf_local_renaming Σ Γ : 
-  All_local_env (lift_typing (fun (Σ : global_env_ext) (Γ : context) (t T : term) =>
-    forall (Δ : PCUICEnvironment.context) (f : nat -> nat),
-    urenaming Δ Γ f -> Σ;;; Δ |- rename f t : rename f T) Σ) Γ ->
-  forall Δ' f, 
-  urenaming Δ' Γ f ->
-  wf_local Σ Δ'.
-Proof.
-  intros. red in X0.
-  induction X.
-  - red in X0.
-  - simpl. destruct t0 as [s Hs].
-    rewrite rename_context_snoc /=. constructor; auto.
-    red. simpl. exists s.
-    eapply (Hs (Δ' ,,, rename_context f Γ0) (shiftn #|Γ0| f)).
-    split => //. 
-    now eapply urenaming_context.
-  - destruct t0 as [s Hs]. red in t1.
-    rewrite rename_context_snoc /=. constructor; auto.
-    * red. exists s.
-      apply (Hs (Δ' ,,, rename_context f Γ0) (shiftn #|Γ0| f)).
-      split=> //. now eapply urenaming_context.
-    * red. apply t1. split => //.
-      now eapply urenaming_context. 
-Qed.*)
-
-Lemma renaming_extP P P' Σ Γ Δ f :
-  P =1 P' ->
-  renaming P Σ Γ Δ f -> renaming P' Σ Γ Δ f.
-Proof.
-  intros hP; rewrite /renaming.
-  intros []; split; eauto.
-  eapply urenaming_ext; eauto. reflexivity.
 Qed.
 
 (** For an unconditional renaming defined on all variables in the source context *)
@@ -3077,10 +1626,10 @@ Proof.
     + eapply cumul_renameP. all: try eassumption.
       * apply hf.
       * pose proof (type_closed _ ht).
-        now eapply closedn_all_free_vars in H.
+        now eapply closedn_on_free_vars in H.
       * pose proof (subject_closed _ htB).
-        now eapply closedn_all_free_vars in H.
-      * pose proof (closed_ctx_all_free_vars P _ (closed_wf_local _ (typing_wf_local ht))).
+        now eapply closedn_on_free_vars in H.
+      * pose proof (closed_ctx_on_free_vars P _ (closed_wf_local _ (typing_wf_local ht))).
         rewrite -{2}(app_context_nil_l Γ).
         eapply on_ctx_free_vars_extend => //.
 Qed.
@@ -3097,18 +1646,6 @@ Proof.
   apply typing_rename_prop.
 Qed.
 
-Lemma urenaming_impl :
-  forall (P P' : nat -> bool) Γ Δ f,
-    (forall i, P' i -> P i) ->
-    urenaming P Δ Γ f ->
-    urenaming P' Δ Γ f.
-Proof.
-  intros P P' Γ Δ f hP h.
-  intros i decl p e.
-  specialize (h i decl (hP _ p) e) as [decl' [h1 [h2 h3]]].
-  exists decl'. split ; [| split ]; eauto.
-Qed.
-
 Lemma typing_rename :
   forall Σ Γ Δ f t A,
     wf Σ.1 ->
@@ -3119,79 +1656,6 @@ Proof.
   intros Σ Γ Δ f t A hΣ hf h.
   eapply (typing_rename_P (fun _ => false)) ; eauto.
 Qed.
-
-Lemma typing_all_free_vars : env_prop
-  (fun Σ Γ t A =>
-    forall P,
-    all_free_vars (closedP #|Γ| P) t ->
-    ∑ Af, (red Σ Γ A Af * all_free_vars (closedP #|Γ| P) Af))
-   (fun Σ Γ =>
-   All_local_env
-   (lift_typing (fun (Σ : global_env_ext) (Γ : context) (t T : term)
-    =>
-    forall P,
-    all_free_vars (closedP #|Γ| P) t ->
-    ∑ Af, (red1 Σ Γ T Af * all_free_vars (closedP #|Γ| P) Af)) Σ) Γ).
-Proof.
-  (*
-  apply typing_ind_env.
-  7:{
-    - intros Σ wfΣ Γ wfΓ t na A B a u X hty ihty ht iht hu ihu P.
-      simpl. move/andP=> [havt havs].
-      destruct (iht _ havt) as [ty [redty hav]].
-      eapply invert_red_prod in redty as [A' [B' [[eq redA] redB]]]. subst ty.
-      move: hav => /= /andP [hA' hB'].
-      eexists (B' {0 := a}); split. 1:admit.
-      eapply all_free_vars_subst=> /=; rewrite ?havs //. }
-  2:{ - intros Σ wfΣ Γ wfΓ n decl isdecl ihΓ P.
-        simpl in * => hn.
-        eexists; split; eauto.
-        eapply (nth_error_All_local_env (n:=n)) in ihΓ.
-        2:{ eapply nth_error_Some_length in isdecl; eauto. }
-        rewrite isdecl in ihΓ. simpl in ihΓ. rewrite /closedP in hn.
-        move: hn; nat_compare_specs => //. intros pn.
-        move: ihΓ. unfold on_local_decl. 
-        destruct decl_body eqn:db;
-        unfold lift_typing; simpl.
-        * intros ih. specialize (ih P).
-          rewrite skipn_length // in ih.
-          rewrite all_free_vars_lift0 //.
-          admit.
-        * admit. }
-
-  13:{
-    - intros Σ wfΣ Γ wfΓ t A B X hwf ht iht htB ihB cum P hav.
-      specialize (iht _ hav) as [Af [redAf havaf]].
-      admit. (* certainly provable *)
-  }*)
-Admitted.
-
-(* 
-Lemma typing_rename_prop' : env_prop
-  (fun Σ Γ t A =>
-    forall Δ f,
-    renaming (closedP #|Γ| xpredT) Σ Δ Γ f ->
-    Σ ;;; Δ |- rename f t : rename f A)
-   (fun Σ Γ =>
-   All_local_env
-   (lift_typing (fun (Σ : global_env_ext) (Γ : context) (t T : term)
-    =>
-    forall P (Δ : PCUICEnvironment.context) (f : nat -> nat),
-    renaming (closedP #|Γ| P) Σ Δ Γ f -> 
-    Σ;;; Δ |- rename f t : rename f T) Σ) Γ).
-Proof.
-  red. intros.
-  destruct (typing_rename_prop Σ wfΣ Γ t T ty) as [? []].
-  split.
-  - eapply on_global_env_impl. 2:eapply f.
-    intros.
-    red in X0. destruct T0; red.
-    * intros.
-      eapply (X0 xpredT).
-      
-
-
-  destruct X. *)
 
 End Renaming.
 
