template-coq/theories/utils/MCPred.v
@@ -1,0 +1,45 @@
+From Coq Require Import List Bool Arith ssreflect ssrbool Morphisms Lia.
+From MetaCoq.Template Require Import MCPrelude MCReflect MCList MCRelations MCProd MCOption.
+From Equations Require Import Equations.
+
+Definition predA {A} (p q : pred A) : pred A := (fun i => p i ==> q i).
+
+(* 
+Definition orP (p q : nat -> bool) (n : nat) : bool :=
+  p n || q n.
+
+Definition conjP (p q : nat -> bool) (n : nat) : bool :=
+  p n && q n.
+
+Definition implP (p q : nat -> bool) (n : nat) : bool :=
+  p n ==> q n. *)
+
+Instance orP_Proper {A} : Proper (`=1` ==> `=1` ==> `=1`) (@predU A).
+Proof.
+  intros f g Hfg f' g' Hfg' i; rewrite /predU /=.
+  now rewrite Hfg Hfg'.
+Qed.
+
+Instance andP_Proper A : Proper (`=1` ==> `=1` ==> `=1`) (@predI A).
+Proof.
+  intros f g Hfg f' g' Hfg' i; rewrite /predI /=.
+  now rewrite Hfg Hfg'.
+Qed.
+
+Instance implP_Proper {A} : Proper (`=1` ==> `=1` ==> `=1`) (@predA A).
+Proof.
+  intros f g Hfg f' g' Hfg' i; rewrite /predA /=.
+  now rewrite Hfg Hfg'.
+Qed.
+
+Lemma orPL (p q : nat -> bool) : predA p (predU p q) =1 xpredT.
+Proof.
+  intros i. rewrite /predA /predU /=.
+  rewrite (ssrbool.implybE (p i)).
+  destruct (p i) => //.
+Qed.
+
+Lemma orPR (p q : nat -> bool) i : q i -> (predU p q) i.
+Proof.
+  rewrite /predU /= => ->; rewrite orb_true_r //.
+Qed.
